\documentclass[11pt,a4paper]{article}
\usepackage{amsmath}
\begin{document}
	\begin{itemize}
		\item \begin{equation}
			(x+y)^2 = x^2 + 2xy + y^2
		\end{equation} 
		\item \begin{equation}
			 E = mc^2
		\end{equation}
		\item $ x^n + y^n = z^n $
		\item
		$(x+y)^3\\ = (x+y)^2(x+y)  $ \\
		$  = (x^2 + 2xy + y^2)(x+y)$ \\
		$ = (x^3 + 2x^2y + xy^2) + (x^2y + 2xy^2 + y^3)$ \\ 
		$ = x^3 + 3x^2y + 3xy^2 + y^3$ \\
		\item $ f(x) = x^2$ \\
		\item $ g(x) = \frac{1}{x} $ 
		\item $ |\alpha + \sqrt{\alpha^2 - \beta^2}| + |\alpha - \sqrt{\alpha^2 - \beta^2}| = |\alpha + \beta| + |\alpha - \beta| $
		
		\item $ F(x) = \int_{b}^{a} \frac{1}{3} x^3 $
		\item $ \frac{\partial x}{\partial y} $
		\item $\lim_{x \to \alpha} f(x)$
		\item $ \tau = x = \frac{1}{3a(1+u^2)^2}  $
		\item $ \sum_{1}^{n} n = 1 + 2 + 3 + ....... + n = n(n+1) /2 = \frac{n^2}{2} + \frac{n}{2}  $
		\item $ \sum_{j=1}^{m} \min_{i=1}^{n} |x_i - y_j| $ \\
		\item $ A = A_1 + A_2 $
		\item $ \begin{bmatrix}
			a & b \\
			c & d
		\end{bmatrix} $
	\end{itemize}
\end{document}